testsuite/tests/coqgen/refproof.v
@@ -1,17 +1,11 @@
 From mathcomp Require Import all_ssreflect.
-Require Import Sint63 cocti_defs test2.
+Require Import Sint63 BinNums ZArith cocti_defs test2.
 
 Fixpoint fact_rec_pos (n : nat) : nat :=
   match n with
   | 0 => 1
   | m.+1 => m.+1 * fact_rec_pos m
   end.
-Print pos_neg_int63.
-Print nat.
-Print to_Z.
-Print BinNums.Z.
-Check Z0.
-Check Zneg 1%sint63.
 
 Definition fact_rec (n : int) : nat := 
   match to_Z n with
@@ -21,7 +15,7 @@ Definition fact_rec (n : int) : nat :=
   end.
 
 Theorem fact_ok h n :
-  inl_inv(snd(fact_for h (n:>int) empty_env)) = fact_rec n.
+  inl_inv(snd(fact_for h n empty_env)) = fact_rec n.
 Proof.
 
 Qed.
